theories/Monad/ContMonad.v
@@ -1,0 +1,43 @@
+Require Import Monad.
+
+Set Implicit Arguments.
+Set Strict Implicit.
+
+Section ContType.
+  Variable Ans : Type.
+
+  Record cont (t : Type) : Type := mkCont
+  { runCont : (t -> Ans) -> Ans }.
+
+  Global Instance Monad_cont : Monad cont :=
+  { ret  := fun _ v => mkCont (fun k => k v)
+  ; bind := fun _ c1 _ c2 => 
+    mkCont (fun k => 
+      runCont c1 (fun t => 
+        match c2 t with
+          | mkCont k' => k' k
+        end))
+  }.
+
+  Global Instance Cont_cont : Cont cont :=
+  { callCC := fun _ _ f => mkCont (fun c => runCont (f (fun x => mkCont (fun _ => c x))) c)
+  }.  
+
+  Variable m : Type -> Type.
+
+  Record contT (t : Type) : Type := mkContT
+  { runContT : (t -> m Ans) -> m Ans }.
+
+  Global Instance Monad_contT (M : Monad m) : Monad contT :=
+  { ret := fun _ x => mkContT (fun k => k x)
+  ; bind := fun _ c1 _ c2 =>
+    mkContT (fun c => 
+      runContT c1 (fun a => runContT (c2 a) c))
+  }.
+
+  Global Instance Cont_contT (M : Monad m) : Cont contT :=
+  { callCC := fun _ _ f => mkContT (fun c => runContT (f (fun x => mkContT (fun _ => c x))) c)
+  }.
+
+
+End ContType.
