theories/Monad/StateMonad.v
@@ -9,7 +9,7 @@ Section StateType.
   Record state (t : Type) : Type := mkState
   { runState : S -> t * S }.
 
-  Instance Monad_state : Monad state :=
+  Global Instance Monad_state : Monad state :=
   { ret  := fun _ v => mkState (fun s => (v, s))
   ; bind := fun _ c1 _ c2 => 
     mkState (fun s => 
@@ -17,7 +17,7 @@ Section StateType.
       runState (c2 v) s)
   }.
 
-  Instance State_state : State S state :=
+  Global Instance State_state : State S state :=
   { get := mkState (fun x => (x,x))
   ; put := fun v => mkState (fun _ => (tt, v))
   }.
@@ -27,7 +27,7 @@ Section StateType.
   Record stateT (t : Type) : Type := mkStateT
   { runStateT : S -> m (t * S)%type }.
 
-  Instance Monad_stateT (M : Monad m) : Monad stateT :=
+  Global Instance Monad_stateT (M : Monad m) : Monad stateT :=
   { ret := fun _ x => mkStateT (fun s => @ret _ M _ (x,s))
   ; bind := fun _ c1 _ c2 =>
     mkStateT (fun s => 
@@ -36,7 +36,7 @@ Section StateType.
         runStateT (c2 v) s))
   }.
 
-  Instance State_stateT (M : Monad m) : State S stateT :=
+  Global Instance State_stateT (M : Monad m) : State S stateT :=
   { get := mkStateT (fun x => ret (x,x))
   ; put := fun v => mkStateT (fun _ => ret (tt, v))
   }.
